QHC-13: new expectation

FY/Logic.v
@@ -14,6 +14,18 @@ Theorem fy_skip: forall n P, hoare_triple n n P <{skip}> P.
 Proof.
 Admitted.
 
+Definition assign_sub n X a (P : Assertion n) : Assertion n :=
+  fun (st : (total_map nat)) => P (X !-> a ; st).
+
+Definition init_sub n (P : Assertion n) : Assertion (n + 1) :=
+  fun (st : (total_map nat)) => pair (fst (P st)) (∣0⟩⟨0∣ ⊗ (snd (P st))).
+
+Definition apply_sub n (U: Unitary n) (P : Assertion n) : Assertion n :=
+  fun (st : (total_map nat)) => pair (fst (P st)) (Mmult (Mmult U† (snd (P st))) U).
+
+Definition apply_boolean n (b: bool_exp) (P : Assertion n) : Assertion n :=
+  fun (st : (total_map nat)) => pair (beval st b = true) (snd (P st)).
+
 Theorem fy_sequence: forall np nq nr P Q R c1 c2, 
     hoare_triple np nq P c1 Q ->
     hoare_triple nq nr Q c2 R ->
@@ -21,16 +33,48 @@ Theorem fy_sequence: forall np nq nr P Q R c1 c2,
 Proof.
 Admitted.
 
-Definition n : nat := 0%nat.
-
-Check Assertion.
-
-(*
-Theorem fy_assign: forall n x e st U, 
-    hoare_triple n n ((x !-> e ;st) -> U) <{ x :=c e }> (st -> U).
+Theorem fy_assign: forall n x e P, 
+    hoare_triple n n (assign_sub n x e P) <{ x :=c e }> P.
 Proof.
 Admitted.
-*)
+
+Theorem fy_init: forall n m P, 
+    hoare_triple n n (init_sub n P) <{ q m := 0 }> P.
+Proof.
+Admitted.
+
+Theorem fy_apply: forall n m G P, 
+    hoare_triple n n (apply_sub n (geval G) P) <{ q m *= G }> P.
+Proof.
+Admitted.
+
+(*TODO*)
+Theorem fy_measure: forall n x m P, 
+    hoare_triple n n P  <{ x :=measQ m }> P.
+Proof.
+Admitted.
+
+Theorem fy_if: forall (n: nat) (b: bool_exp) (c1 c2: com) P Q, 
+    hoare_triple n n (apply_boolean n b P) c1 Q ->
+    hoare_triple n n (apply_boolean n <{ ~ b }> P) c2 Q ->
+    hoare_triple n n P <{ if b then c1 else c2 end }> Q.
+Proof.
+Admitted.
+
+Theorem fy_while: forall n b c P,
+    hoare_triple n n (apply_boolean n b P) c P ->
+    hoare_triple n n P <{ while b do c end }> (apply_boolean n <{ ~ b }> P).
+Proof.
+Admitted.
+
+Theorem fy_weakness: forall n c st P Q P' Q',
+    hoare_triple n n P c Q ->
+    weaker n n n st P' P ->
+    weaker n n n st Q Q' ->
+    hoare_triple n n P' c Q'.
+Proof.
+Admitted.
 
 
 
+ 
