FY/Assertion.v
@@ -3,20 +3,28 @@ From Coq Require Import Strings.String.
 From FY Require Export Utils.
 Import ListNotations.
 
-Definition Assertion (nq: nat) := (total_map nat) -> (Unitary nq).
+Definition Assertion (n: nat) := pair Prop (Unitary n).
 
+(*  *)
 Fixpoint Expectation (ns na : nat) 
-     (state: list ((total_map nat)*(Unitary ns))) 
+     (state: list ((total_map nat) * (Unitary ns))) 
      (assertion: Assertion na) : C :=
     match state with
     | [] => 0%C
     | st :: l => 
-        Cplus 
-            (trace (Mmult (kron (snd st) (I (ns - na))) 
-            (assertion (fst st)))) 
-            (Expectation ns na l assertion)
+        match (fst (assertion (fst st))) with
+         | True => Cplus 
+                    (trace (Mmult (kron (snd st) (I (ns - na))) 
+                    (snd (assertion (fst st))))) 
+                    (Expectation ns na l assertion)
+        end
     end
 .
+
+
+
+
+
 
 Definition weaker (ns na1 na2 : nat) (state: list ((total_map nat)*(Unitary ns))) (assertion1: Assertion na1) (assertion2: Assertion na2) : Prop :=
     Cnorm (Expectation ns na1 state assertion1) <= Cnorm (Expectation ns na2 state assertion2).
