FY/Examples.v
@@ -9,13 +9,22 @@ From FY Require Export Semantics.
 Definition X : string := "X".
 
 Definition Prog1 : com :=
-  <{ q 0 :=q 0;
+  <{ q 0 := 0;
      q 0 *= GH;
      X :=measQ 0%nat }>.
 Print Prog1.
 
+(* ENONTRA BOM EXEMPLOS PARA APRESENTAÇÃO*)
+(* () -> ∣0⟩⟨0∣ . I *)
+(* 
+(X -> 0) ->  1/sqrt(2)[[1, -1], [1, 1]]
+(X -> 1) ->  1/sqrt(2)[[1, -1], [1, 1]]
+
+() -> (X < 0.5) * (I 2)
+*)
+
 Definition Prog2 : com :=
-  <{ q 0 :=q 0;
+  <{ q 0 := 0;
      q 0 *= GH;
      X :=measQ 0%nat;
      if BEq X 2%nat then
@@ -26,15 +35,31 @@ Definition Prog2 : com :=
 Print Prog2.
 
 Definition Prog3 : com :=
-  <{ q 0%nat :=q 0 }>.
+  <{ q 0 := 0;
+     q 0 *= GH }>.
+
+
+Definition Prog4 : com :=
+  <{ q 0%nat := 0 }>.
+
+Definition zero := 0%nat.
+
+Definition Prog5 : com :=
+  <{ X :=c APlus 0%nat 1%nat }>.
 
 Theorem state_eval_1: ceval Prog1 [((_ !-> 0%nat), I 2)] [((X !-> 0%nat ; _ !-> 1%nat), H) ; ((X !-> 1%nat; _ !-> 1%nat), H)].
 Proof.
+  eapply E_Seq.
+  apply E_Init.
+  eapply E_Seq.
+  apply E_App.
+  apply E_Meas.
   apply E_Seq with [((X !-> 0%nat ; _ !-> 0%nat), H) ; ((X !-> 1%nat; _ !-> 0%nat), H)].
+
 Admitted.
 
 
-Theorem state_eval_3: ceval <{ q 0%nat :=q 0 }> [((_ !-> 0%nat), I 2)] [((_ !-> 0%nat), ∣0⟩⟨0∣)].
+Theorem state_eval_3: ceval <{ q 0%nat := 0 }> [((_ !-> 0%nat), I 2)] [((_ !-> 0%nat), ∣0⟩⟨0∣)].
 Proof.
 Admitted.
 
